Add flatten non-recursive line-ok corollaries and expose stackIsSkip

Flapjack/Compiler/Backend/StackToLab.lean
@@ -32,7 +32,7 @@ abbrev FlatLine (Memop Addr Cmp RegImm MlString AsmInst Word : Type) :=
 private def findLab (index : Nat) (labs : List Nat) : Nat :=
   (labs[index]?).getD 0
 
-private def isSkip {Inst Cmp RegImm Binop Memop Addr MlString : Type} :
+def stackIsSkip {Inst Cmp RegImm Binop Memop Addr MlString : Type} :
     Prog Inst Cmp RegImm Binop Memop Addr MlString → Bool
   | .skip => true
   | _ => false
@@ -61,12 +61,12 @@ def flatten {Inst Cmp RegImm Binop Memop Addr MlString AsmInst Word : Type}
     | .ite condition register right thenBranch elseBranch =>
         let (xs, nr1, next) := flatten ops zero false thenBranch sectionId next conts breaks
         let (ys, nr2, next) := flatten ops zero false elseBranch sectionId next conts breaks
-        if isSkip thenBranch && isSkip elseBranch then
+        if stackIsSkip thenBranch && stackIsSkip elseBranch then
           ([], false, next)
-        else if isSkip thenBranch then
+        else if stackIsSkip thenBranch then
           ([.labAsm (.jumpCmp condition register right (.lab sectionId next)) zero [] 0] ++
             ys ++ [.label sectionId next 0], false, next + 1)
-        else if isSkip elseBranch then
+        else if stackIsSkip elseBranch then
           ([.labAsm (.jumpCmp (ops.negate condition) register right (.lab sectionId next)) zero [] 0] ++
             xs ++ [.label sectionId next 0], false, next + 1)
         else if nr1 then
